add sketch of top down

dafny/lcf/main.dfy
@@ -72,6 +72,8 @@ datatype Thm = Thm(val : Term, ghost p : Proof) {
 function mk_thm(rs : RuleSet, i : nat, s : Subst, args : seq<Thm>) : (res : Result<Thm>)
         requires i < |rs| 
         requires forall j :: 0 <= j < |args| ==> args[j].wf(rs) 
+        ensures rs[i].complete_subst(s) && |args| == |rs[i].body| && (forall j :: 0 <= j < |args| ==> args[j].val == rs[i].subst(s).body[j]) 
+            ==> res.Ok?
         ensures res.Ok? ==> rs[i].complete_subst(s) && res.val.wf(rs) && res.val.val == rs[i].subst(s).head {
             var r := rs[i];
             if |args| == |r.body| && r.complete_subst(s) && (forall j :: 0 <= j < |args| ==> args[j].val == r.subst(s).body[j]) then
@@ -81,14 +83,100 @@ function mk_thm(rs : RuleSet, i : nat, s : Subst, args : seq<Thm>) : (res : Resu
             else Err
     }
 
-///// Below here, everything is untrusted /////
+
+//// Extremely toy top-down ////
+
+function collect_result<A>(xs : seq<Result<A>>) : (res:Result<seq<A>>)
+    ensures res.Ok? ==> |res.val| == |xs| && forall j :: 0 <= j < |xs| ==> xs[j].Ok? && res.val[j] == xs[j].val
+    {
+        if xs == [] then Ok([]) else
+        if xs[0].Ok? then 
+            match collect_result(xs[1..])
+                case Ok(ys) => Ok([xs[0].val] + ys)
+                case Err => Err
+        else Err
+    }
+
+function unify_vars(s : seq<string>, t : seq<string>) : (res : Result<map<string, string>>)
+    ensures res.Ok? ==> |s| == |t| && forall i :: 0 <= i < |s| ==> s[i] in res.val && res.val[s[i]] == t[i] 
+{
+    if |s| != |t| then Err else 
+    if s == [] then Ok(map[]) else
+        match unify_vars(s[1..], t[1..]) 
+            case Err => Err
+            case Ok(sbst) => 
+                if (s[0] !in sbst) || (sbst[s[0]] == t[0]) then 
+                    Ok(sbst[s[0] := t[0]])
+                else Err 
+}
+
+function unify(r : Term, g : Term) : (res : Result<Subst>)
+    ensures res.Ok? ==> r.complete_subst(res.val) && r.subst(res.val) == g
+    {
+        match (r, g)
+            case (Const(v1), Const(v2)) => if v1 == v2 then Ok(map[]) else Err
+            case (App(f1, args1), App(f2, args2)) => 
+                if f1 == f2 then 
+                    match unify_vars(args1, args2)
+                        case Ok(s) => 
+                            assert seq(|args1|, i requires 0 <= i < |args1| => s[args1[i]]) == args2;
+                            Ok(s)
+                        case Err => Err
+                else Err
+            case _ => Err
+    }
+
+function find_unify(rs : RuleSet, goal : Term) : (res:Result<(nat, Subst)>)
+    ensures res.Ok? ==> res.val.0 < |rs| && unify(rs[res.val.0].head, goal) == Ok(res.val.1)
+    {
+        if rs == [] then Err else 
+        match unify(rs[0].head, goal)
+            case Err => 
+                (match find_unify(rs[1..], goal)
+                    case Err => Err
+                    case Ok((i, s)) => Ok((i+1, s))
+                )
+            case Ok(res) => Ok((0,res))
+    }
+
+
+
+// TODO: 
+// - only tries the first matching rule it finds
+// - only works on rules without existential quantification (e.g., more variables in the body) 
+// - does not memoize subgoals
+function top_down(rs : RuleSet, goal : Term, bound : nat) : (res:Result<Thm>)
+    ensures res.Ok? ==> res.val.wf(rs) && res.val.val == goal
+
+    decreases bound {
+        if bound == 0 then Err else
+        // Find a rule that unifies with the goal; obtain rule index i, substitution s
+        match find_unify(rs, goal)
+            case Err => Err
+            case Ok((i, s)) => 
+                var rule := rs[i];
+                // If the substitution s is actually good for the _entire_ rule,
+                if rule.complete_subst(s) then
+                    // Call top_down recursively on the rule arguments; fail if top down fails on any of them
+                    var arg_thms_result := collect_result(seq(|rule.body|, j requires 0 <= j < |rule.body| =>
+                        var subgoal := rule.subst(s).body[j];
+                        top_down(rs, subgoal, bound-1)
+                    ));
+                    if arg_thms_result.Ok? then
+                        // We have actually proven that mk_thm will now succeed; get the theorem and return it
+                        Ok(mk_thm(rs, i, s, arg_thms_result.val).val)
+                    else Err
+                else Err
+
+}
+
+///// Also works bottom up ////// 
 
 function find_new_subst(rs : RuleSet, thms : seq<Thm>) : (res : Result<(nat, Subst, seq<Thm>)>)
     requires forall i :: 0 <= i < |thms| ==> thms[i].wf(rs)
     ensures res.Ok? ==> 
         res.val.0 < |rs| &&
         forall j :: 0 <= j < |res.val.2| ==> res.val.2[j].wf(rs)
-
         
 function bottom_up(rs : RuleSet, acc : seq<Thm>, bound : nat) : seq<Thm> 
     requires forall i :: 0 <= i < |acc| ==> acc[i].wf(rs)
